updates

generic/Zeta.GenericVerifier.fst
@@ -1,7 +1,98 @@
 module Zeta.GenericVerifier
 
+open Zeta.SeqIdx
+open FStar.Classical
+
+let not_contains_app_key (#vspec:_)
+  (vtls: vspec.vtls_t{vspec.valid vtls})
+  (s: vspec.slot_t)
+  : bool
+  = not (contains_app_key vtls s)
+
+let contains_only_app_keys_comp (#vspec:_) (vtls: vspec.vtls_t{vspec.valid vtls}) (ss: S.seq vspec.slot_t)
+  : b:bool {b <==> contains_only_app_keys vtls ss}
+  = not (exists_elems_with_prop_comp (not_contains_app_key vtls) ss)
+
+#push-options "--fuel 0 --ifuel 1 --query_stats"
+
+let rec search_level_2_aux (#vspec:_) (vtls: vspec.vtls_t{vspec.valid vtls})
+  (ss: S.seq vspec.slot_t{contains_only_app_keys vtls ss})
+  (i1: SA.seq_index ss)
+  (l: nat {l <= S.length ss})
+  : Tot(o:option nat
+    { None = o /\ (forall i2. i2 < l ==> i1 <> i2 ==> to_app_key vtls (S.index ss i1) <> to_app_key vtls (S.index ss i2)) \/
+      Some? o /\ (let i2 = Some?.v o in
+                 i2 < l /\ i1 <> i2 /\
+                 to_app_key vtls (S.index ss i1) = to_app_key vtls (S.index ss i2))})
+    (decreases l)
+  = if l = 0 then None
+    else (
+      let l' = l - 1 in
+      let o = search_level_2_aux vtls ss i1 l' in
+      if l' <> i1 && to_app_key vtls (S.index ss i1) = to_app_key vtls (S.index ss l') then
+        Some l'
+      else if Some? o then
+        o
+      else (
+        let aux (i2:_)
+          : Lemma (ensures (i2 < l ==> i1 <> i2 ==>
+                            to_app_key vtls (S.index ss i1) <> to_app_key vtls (S.index ss i2)))
+          = if i2 < l' && i1 <> i2 then
+            eliminate
+            forall i2. i2 < l' ==> i1 <> i2 ==> to_app_key vtls (S.index ss i1) <> to_app_key vtls (S.index ss i2)
+            with i2
+        in
+        forall_intro aux;
+        None
+      )
+    )
+
+let search_level_2 (#vspec:_) (vtls: vspec.vtls_t{vspec.valid vtls})
+  (ss: S.seq vspec.slot_t{contains_only_app_keys vtls ss})
+  (i1: SA.seq_index ss)
+  : (o:option nat
+    { None = o /\ (forall i2. i1 <> i2 ==> to_app_key vtls (S.index ss i1) <> to_app_key vtls (S.index ss i2)) \/
+      Some? o /\ (let i2 = Some?.v o in
+                 i1 <> i2 /\ i2 < S.length ss /\
+                 to_app_key vtls (S.index ss i1) = to_app_key vtls (S.index ss i2))})
+  = search_level_2_aux vtls ss i1 (S.length ss)
+
+let rec search_level_1_aux (#vspec:_) (vtls: vspec.vtls_t{vspec.valid vtls})
+  (ss: S.seq vspec.slot_t{contains_only_app_keys vtls ss})
+  (l: nat{l <= S.length ss})
+  : Tot(o:option (nat * nat)
+    { None = o /\ (forall i1 i2. i1 < l ==> i1 <> i2 ==>
+                           to_app_key vtls (S.index ss i1) <> to_app_key vtls (S.index ss i2)) \/
+      Some? o /\ (let i1,i2 = Some?.v o in
+                 i1 < l /\ i1 <> i2 /\ i2 < S.length ss /\
+                 to_app_key vtls (S.index ss i1) = to_app_key vtls (S.index ss i2))
+    })
+    (decreases l)
+  = if l = 0 then None
+    else (
+      let i1 = l - 1 in
+      let ol' = search_level_2 vtls ss i1 in
+      if Some? ol' then (
+        admit()
+      )
+      else
+
+      admit()
+    )
+
+let search_level_1 (#vspec:_) (vtls: vspec.vtls_t{vspec.valid vtls})
+  (ss: S.seq vspec.slot_t{contains_only_app_keys vtls ss})
+  : Tot(o:option (nat * nat)
+    { None = o /\ (forall i1 i2. i1 <> i2 ==>
+                           to_app_key vtls (S.index ss i1) <> to_app_key vtls (S.index ss i2)) \/
+      Some? o /\ (let i1,i2 = Some?.v o in
+                 i1 <> i2 /\ i2 < S.length ss /\ i1 < S.length ss /\
+                 to_app_key vtls (S.index ss i1) = to_app_key vtls (S.index ss i2))
+    })
+  = search_level_1_aux vtls ss (S.length ss)
+
 let contains_distinct_app_keys_comp
   (#vspec:_) (vtls: vspec.vtls_t{vspec.valid vtls}) (ss: S.seq vspec.slot_t)
   : b:bool {b <==> contains_distinct_app_keys vtls ss}
-  = admit()
-
+  = contains_only_app_keys_comp vtls ss &&
+    None = search_level_1 vtls ss
